theories/base_logic/lib/wsat.v
@@ -936,60 +936,6 @@ Qed.
 
 End schema_test_bupd.
 
-Section schema_test_fupd.
-Context `{!invG Σ}.
-Implicit Types P : iProp Σ.
-
-Definition bi_sch_False : bi_schema := bi_sch_pure False.
-
-Definition bi_sch_except_0 (P: bi_schema) : bi_schema :=
-  bi_sch_or (bi_sch_later (bi_sch_False)) P.
-
-Definition bi_sch_bupd_wand (P1 P2: bi_schema) :=
-  bi_sch_wand P1 (bi_sch_bupd P2).
-
-Definition bi_sch_fupd E1 E2 (P: bi_schema) : bi_schema :=
-  bi_sch_bupd_wand
-    (bi_sch_sep (bi_sch_wsat) (bi_sch_ownE E1))
-    (bi_sch_except_0 (bi_sch_sep (bi_sch_wsat)
-                                (bi_sch_sep (bi_sch_ownE E2) P))).
-
-Lemma bi_sch_fupd_interp E1 E2 lvl Qs Qs_mut Psch P:
-  bi_schema_interp lvl Qs Qs_mut Psch = P →
-  bi_schema_interp lvl Qs Qs_mut (bi_sch_fupd E1 E2 Psch) =
-    (wsat lvl ∗ ownE E1 ==∗ ◇ (wsat lvl ∗ ownE E2 ∗ P))%I.
-Proof.
-  intros Heq.
-  rewrite ?bi_schema_interp_unfold //=.
-  do 11 (rewrite {1}bi_schema_interp_unfold //=).
-  rewrite Heq. rewrite ?bi_schema_interp_unfold //=.
-Qed.
-
-Definition ownI_fupd lvl i E1 E2 P :=
-  ownI lvl i (bi_sch_fupd E1 E2 (bi_sch_var_fixed O)) (list_to_vec [P]).
-
-Lemma ownI_fupd_alloc lvl E1 E2 φ P :
-  (∀ E : gset positive, ∃ i, i ∉ E ∧ φ i) →
-  wsat (S lvl) ∗ (wsat lvl ∗ ownE E1 ==∗ ◇ (wsat lvl ∗ ownE E2 ∗ ▷ P))
-       ==∗ ∃ i, ⌜φ i⌝ ∗ wsat (S lvl) ∗ ownI_fupd lvl i E1 E2 P.
-Proof.
-  iIntros (?) "HwP". iApply ownI_alloc_nomut; eauto.
-  erewrite bi_sch_fupd_interp; eauto.
-  rewrite ?bi_schema_interp_unfold //=.
-Qed.
-
-Lemma ownI_fupd_open lvl E1 E2 i P :
-  wsat (S lvl) ∗ ownI_fupd lvl i E1 E2 P ∗ ownE {[i]} ⊢
-  wsat (S lvl) ∗ (wsat lvl ∗ ownE E1 ==∗ ◇ (wsat lvl ∗ ownE E2 ∗ ▷ P)) ∗ ownD {[i]}.
-Proof.
-  iIntros "Hw". iDestruct (ownI_open with "Hw") as "($&HP&$)".
-  iDestruct "HP" as (??) "(HP&_)".
-  erewrite bi_sch_fupd_interp; eauto.
-  rewrite ?bi_schema_interp_unfold //=.
-Qed.
-
-End schema_test_fupd.
-
 Section schema_test_mut.
 Context `{!invG Σ}.
 Implicit Types P Q : iProp Σ.
